Tealeaves/Examples/VariadicLet/Syntax.v
@@ -1,0 +1,237 @@
+From Tealeaves Require Export
+  Examples.VariadicLet.Terms.
+
+#[local] Generalizable Variables G A B C.
+#[local] Set Implicit Arguments.
+
+Fixpoint binddt_term
+           (G : Type -> Type) `{Map G} `{Pure G} `{Mult G}
+           {v1 v2 : Type}
+           (f : nat * v1 -> G (term v2))
+           (t : term v1) : G (term v2) :=
+  match t with
+  | tvar v => f (0, v)
+  | letin defs body =>
+      pure (@letin v2) <⋆>
+      ((fix F ls :=
+      match ls with
+      | nil => pure nil
+      | cons d0 drest =>
+          pure cons <⋆> binddt_term f d0 <⋆> F drest
+      end) defs) <⋆> binddt_term (f ⦿ List.length defs) body
+  | app t1 t2 =>
+      pure (@app v2) <⋆> binddt_term f t1 <⋆> binddt_term f t2
+  end.
+
+#[export] Instance Binddt_Lam: Binddt nat term term := @binddt_term.
+
+Lemma binddt_rw_letin: forall `{Applicative G} (v1 v2 : Type)
+                         (l : list (term v1)) (body: term v1),
+  forall f : nat * v1 -> G (term v2),
+    binddt f (letin l body) =
+      pure (@letin v2) <⋆> traverse (binddt f) l <⋆>
+        binddt (f ⦿ List.length l) body.
+Proof.
+  intros.
+  destruct l.
+  - cbn.
+    change 0 with (Ƶ:nat).
+    rewrite preincr_zero.
+    reflexivity.
+  - cbn.
+    repeat fequal.
+    induction l.
+    + reflexivity.
+    + cbn. rewrite IHl.
+      reflexivity.
+Qed.
+
+Lemma binddt_helper_letin
+        `{Applicative G2}
+        B C (l : list (term B))
+        (g : nat * B -> G2 (term C)):
+  binddt g ∘ letin (v:=B) l =
+    (precompose (binddt (g ⦿ List.length l)) ∘ ap G2)
+      (pure (letin (v:=C)) <⋆> (traverse (binddt g) l)).
+Proof.
+  unfold precompose, compose.
+  ext body.
+  rewrite binddt_rw_letin.
+  reflexivity.
+Qed.
+
+Lemma binddt_helper_letin2
+        `{Applicative G2}
+        A B C (l : list (term A))
+    (g : nat * B -> G2 (term C)):
+  compose (binddt_term g) ∘ letin (v:=B) ∘ toMake_mono list l (term B) =
+    ((compose (precompose (binddt_term (g ⦿ List.length l)) ∘ ap G2) ∘
+             precompose (traverse (T := list) (binddt_term g)) ∘
+             ap G2 ∘ pure (F := G2)) (letin (v:=C))) ∘ toMake_mono list l (term B).
+Proof.
+  intros.
+  Check compose (binddt_term g) ∘ letin (v:=B) ∘ toMake list l (term B).
+  (* : Vector.t (term B) (length_gen l) -> term B -> G2 (term C) *)
+  Check
+    (compose (precompose (binddt_term g) ∘ ap G2) ∘
+             precompose (traverse (T := list) (binddt_term g)) ∘
+             ap G2 ∘ pure (F := G2)) (letin (v:=C)).
+  (* : list (term B) -> term B -> G2 (term C) *)
+  Check
+    ((compose (precompose (binddt_term g) ∘ ap G2) ∘
+             precompose (traverse (T := list) (binddt_term g)) ∘
+             ap G2 ∘ pure (F := G2)) (letin (v:=C))) ∘ toMake list l (term B).
+  ext l'.
+  change_left (binddt_term g ∘ letin (toMake_mono list l (term B) l')).
+  ext body.
+
+  rewrite binddt_helper_letin.
+  rewrite length_helper_mono.
+  reflexivity.
+Qed.
+
+Theorem dtm1_lam:
+  forall `{Applicative G} (A B : Type),
+  forall f : nat * A -> G (term B),
+    binddt f ∘ ret  = f ∘ ret (T := (nat ×)).
+Proof.
+  reflexivity.
+Qed.
+
+Theorem dtm2_term : forall A : Type,
+    binddt (T := term) (U := term)
+           (G := fun A => A) (ret (T := term) ∘ extract (W := (nat ×))) = @id (term A).
+Proof.
+  intros. ext t.
+  induction t using term_mut_ind2.
+  - cbn. reflexivity.
+  - rewrite binddt_rw_letin.
+    rewrite extract_preincr2.
+    rewrite IHt.
+    unfold_ops @Pure_I; unfold id.
+    fequal.
+    apply (traverse_respectful_id (T := list)).
+    assumption.
+  - cbn.
+    rewrite IHt1, IHt2.
+    reflexivity.
+Qed.
+
+Theorem dtm3_term:
+  forall `{Applicative G1} `{Applicative G2},
+  forall `(g : nat * B -> G2 (term C)) `(f : nat * A -> G1 (term B)),
+    map (binddt g) ∘ binddt f = binddt (G := G1 ∘ G2) (g ⋆7 f).
+Proof.
+  intros. ext t.
+  generalize dependent g.
+  generalize dependent f.
+  assert (Functor G1) by (now inversion H2).
+  assert (Functor G2) by (now inversion H6).
+  unfold compose at 1.
+  induction t using term_mut_ind2; intros f g.
+  - cbn.
+    change (preincr g 0) with (preincr g Ƶ).
+    now rewrite preincr_zero.
+  - do 2 rewrite binddt_rw_letin.
+    pose (IHt' := IHt (f ⦿ List.length defs) (g ⦿ List.length defs)).
+    rewrite kc7_preincr in IHt'.
+    (* left *)
+    rewrite map_ap.
+    rewrite map_ap.
+    rewrite app_pure_natural.
+    erewrite traverse_repr;
+      try typeclasses eauto.
+    rewrite <- ap4.
+    rewrite ap2.
+    rewrite ap2.
+    rewrite binddt_helper_letin2.
+    rewrite <- map_to_ap.
+    rewrite <- (fun_map_map (F := G1)).
+    unfold compose at 1.
+    rewrite (map_to_ap (toMake_mono list defs _)).
+    rewrite <- (traverse_repr list G1 defs (term B) (binddt f)).
+    rewrite (map_to_ap).
+    (* right *)
+    unfold_ops @Pure_compose.
+    assert (Heqdefs: traverse (binddt (G := G1 ∘ G2) (g ⋆7 f)) defs =
+              map (F := G1)
+                  (traverse (T := list) (binddt (G := G2) g))
+                  (traverse (T := list) (binddt (G := G1) f) defs)).
+    { compose near defs on right.
+      rewrite traverse_traverse.
+      all: try typeclasses eauto.
+      apply traverse_respectful.
+      typeclasses eauto.
+      symmetry.
+      now apply IHdefs. }
+    #[local] Set Keyed Unification.
+    rewrite_strat innermost (terms (ap_compose2 G2 G1)).
+    rewrite app_pure_natural.
+    rewrite Heqdefs.
+    rewrite <- ap_map.
+    rewrite app_pure_natural.
+    rewrite_strat innermost (terms (ap_compose2 G2 G1)).
+    rewrite map_ap.
+    rewrite app_pure_natural.
+    rewrite <- IHt'.
+    rewrite <- ap_map.
+    rewrite map_ap.
+    rewrite app_pure_natural.
+    reflexivity.
+  - cbn.
+    rewrite map_ap.
+    rewrite map_ap.
+    rewrite app_pure_natural.
+    unfold_ops @Pure_compose.
+    rewrite_strat innermost (terms (ap_compose2 G2 G1)).
+    rewrite app_pure_natural.
+    rewrite <- IHt1.
+    rewrite <- ap_map.
+    rewrite app_pure_natural.
+    rewrite_strat innermost (terms (ap_compose2 G2 G1)).
+    rewrite map_ap.
+    rewrite app_pure_natural.
+    rewrite <- IHt2.
+    rewrite <- ap_map.
+    rewrite map_ap.
+    rewrite app_pure_natural.
+    reflexivity.
+    #[local] Unset Keyed Unification.
+Qed.
+
+Theorem dtm4_stlc :
+  forall (G1 G2 : Type -> Type) (H1 : Map G1) (H2 : Mult G1) (H3 : Pure G1) (H4 : Map G2) (H5 : Mult G2) (H6 : Pure G2)
+    (ϕ : forall A : Type, G1 A -> G2 A),
+    ApplicativeMorphism G1 G2 ϕ ->
+    forall (A B : Type) (f : nat * A -> G1 (term B)),
+      ϕ (term B) ∘ binddt f = binddt (ϕ (term B) ∘ f).
+Proof.
+  intros. ext t.
+  inversion H.
+  generalize dependent f.
+  unfold compose at 1.
+  induction t using term_mut_ind2; intro f. (* .unfold *)
+  - reflexivity.
+  - do 2 rewrite binddt_rw_letin.
+    repeat rewrite ap_morphism_1.
+    rewrite appmor_pure.
+    rewrite IHt.
+    change (ϕ (list (term B)) (traverse (binddt f) defs))
+      with ((ϕ (list (term B)) ∘ traverse (binddt f)) defs).
+    rewrite (trf_traverse_morphism).
+    assert (Heqdefs: (traverse (ϕ (term B) ∘ binddt f) defs) =
+                       traverse (binddt (ϕ (term B) ∘ f)) defs).
+    { apply traverse_respectful.
+      typeclasses eauto.
+      intros.
+      unfold compose.
+      now apply IHdefs. }
+    rewrite Heqdefs.
+    reflexivity.
+  - cbn.
+    repeat rewrite ap_morphism_1.
+    rewrite appmor_pure.
+    rewrite IHt1.
+    rewrite IHt2.
+    reflexivity.
+Qed.
